modélisation Isabelle/sync-mod/SyncModProof.thy
@@ -6,7 +6,7 @@ definition HOMachine_to_Algorithm :: "(Proc, pstate, SendVal) HOMachine \<Righta
 "HOMachine_to_Algorithm mach = \<lparr> CinitState = CinitState mach, sendMsg = sendMsg mach, CnextState = CnextState mach \<rparr>"
 
 
-definition monovalent where
+definition monovalent :: "(nat \<Rightarrow> Proc \<Rightarrow> pstate proc_state) \<Rightarrow> nat \<Rightarrow> nat \<Rightarrow> bool" where
 "monovalent rho v n \<equiv> \<forall>p ss st. rho n p = Active ss \<longrightarrow> rho (Suc n) p = Active st \<longrightarrow> x st = v"
 
 (*lemma A1 : assumes "rho r p = Active s"
@@ -21,42 +21,6 @@ proof (rule+)
     show "x st = 0"
     proof -
         *)
-lemma sending : assumes run:"HORun (HOMachine_to_Algorithm (k_mod.SyncMod_HOMachine k)) rho HO" (is "HORun ?A rho HO")
-assumes "(HOrcvdMsgs ?A p (HO (Suc r) p) (rho r)) q = Content (Val v)" (is "?msgs q = _")
-shows "\<exists>s. rho r q = Active s \<and> x s = v"
-proof (cases "rho r q")
-    case Aslept
-    hence "?msgs q = (if q \<in> HO (Suc r) p then Bot else Void)" using HOrcvdMsgs_def[of ?A p "HO (Suc r) p" "rho r"] by auto
-    thus "\<exists>s. rho r q = Active s \<and> x s = v" using \<open>?msgs q = Content (Val v)\<close> by auto
-next
-    case (Active sq)
-    have "sendMsg ?A q p sq = Val (x sq)" using HOrcvdMsgs_def[of ?A p "HO (Suc r) p" "rho r"] \<open>?msgs q = Content (Val v)\<close>
-        by (simp add: Active HOMachine_to_Algorithm_def k_mod.SyncMod_HOMachine_def k_mod.SyncMod_sendMsg_def)
-    hence "k_mod.SyncMod_sendMsg k q p sq = Val (x sq)"
-        using HOMachine_to_Algorithm_def k_mod.SyncMod_HOMachine_def by 
-        (simp add: \<open>\<And>k. k_mod.SyncMod_HOMachine k \<equiv> \<lparr>CinitState = \<lambda>p st crd. k_mod.SyncMod_initState k p st,
-        sendMsg = k_mod.SyncMod_sendMsg k, CnextState = \<lambda>p st msgs crd. k_mod.SyncMod_nextState k p st msgs,
-        HOcommPerRd = k_mod.SyncMod_commPerRd, HOcommGlobal = k_mod.SyncMod_commGlobal,
-        HOcommSchedule = k_mod.SyncMod_commSchedule\<rparr>\<close>)
-    hence "?msgs q = Content (Val (x sq))" using HOrcvdMsgs_def[of ?A p "HO (Suc r) p" "rho r"] \<open>?msgs q = Content (Val v)\<close>
-        by (simp add: Active \<open>sendMsg (HOMachine_to_Algorithm (k_mod.SyncMod_HOMachine k)) q p sq = Val (x sq)\<close>)
-    hence "rho r q = Active sq \<and> x sq = v"
-        using \<open>rho r q = Active sq\<close> \<open>?msgs q = Content (Val v)\<close> k_mod.SyncMod_sendMsg_def[of k q p sq] by auto
-    thus "\<exists>s. rho r q = Active s \<and> x s = v"  by auto
-qed
-
-lemma transition : assumes s_def:"rho r p = Active s"
-and ss_def:"rho (Suc r) p = Active ss"
-and run:"HORun (HOMachine_to_Algorithm (k_mod.SyncMod_HOMachine k)) rho HO" (is "HORun ?A _ _")
-shows "k_mod.SyncMod_nextState k p s (HOrcvdMsgs ?A p (HO (Suc r) p) (rho r)) ss" (is "k_mod.SyncMod_nextState  _ _ _ ?msgs _")
-proof -
-    have "CHOnextConfig ?A (rho r) (HO (Suc r)) (\<lambda>w. undefined) (rho (Suc r))" using run by (simp add:HORun_def CHORun_def)
-    then obtain sss where "rho (Suc r) p = Active sss \<and> CnextState ?A p s ?msgs undefined sss" 
-        using CHOnextConfig_def[of ?A "rho r" "HO (Suc r)" "\<lambda>w. undefined" "rho (Suc r)"] s_def by fastforce
-    hence "CnextState ?A p s ?msgs undefined ss" using ss_def by auto
-    thus ?thesis using HOMachine_to_Algorithm_def k_mod.SyncMod_HOMachine_def[of k] by (simp add:k_mod.simp_nextState)
-qed
-
 lemma stating : assumes "0 < n \<longrightarrow> rho (n-1) p = Aslept"
 and run:"HORun (HOMachine_to_Algorithm (k_mod.SyncMod_HOMachine k)) rho HO" (is "HORun ?A _ _")
 and "rho n p = Active s"
@@ -79,7 +43,68 @@ proof -
         using \<open>x s  = k\<close> by auto
 qed
 
+lemma sending : assumes run:"HORun (HOMachine_to_Algorithm (k_mod.SyncMod_HOMachine k)) rho HO" (is "HORun ?A rho HO")
+assumes "(HOrcvdMsgs ?A p (HO (Suc (Suc r)) p) (rho (Suc r))) q = Content (Val v)" (is "?msgs q = _")
+shows "\<exists>s ss. rho r q = Active s \<and> rho (Suc r) q = Active ss \<and> x ss = v"
+proof (cases "rho (Suc r) q")
+    case Aslept
+    hence "?msgs q = (if q \<in> HO (Suc (Suc r)) p then Bot else Void)"
+        using HOrcvdMsgs_def[of ?A p "HO (Suc (Suc r)) p" "rho (Suc r)"] by auto
+    thus "\<exists>s ss. rho r q = Active s \<and> rho (Suc r) q = Active ss \<and> x ss = v" using \<open>?msgs q = Content (Val v)\<close> by auto
+next
+    case (Active sq)
+    have "sendMsg ?A q p sq = Val (x sq)"
+        using HOrcvdMsgs_def[of ?A p "HO (Suc (Suc r)) p" "rho (Suc r)"] \<open>?msgs q = Content (Val v)\<close>
+        by (simp add: Active HOMachine_to_Algorithm_def k_mod.SyncMod_HOMachine_def k_mod.SyncMod_sendMsg_def)
+    hence "k_mod.SyncMod_sendMsg k q p sq = Val (x sq)"
+        using HOMachine_to_Algorithm_def k_mod.SyncMod_HOMachine_def by 
+        (simp add: \<open>\<And>k. k_mod.SyncMod_HOMachine k \<equiv> \<lparr>CinitState = \<lambda>p st crd. k_mod.SyncMod_initState k p st,
+        sendMsg = k_mod.SyncMod_sendMsg k, CnextState = \<lambda>p st msgs crd. k_mod.SyncMod_nextState k p st msgs,
+        HOcommPerRd = k_mod.SyncMod_commPerRd, HOcommGlobal = k_mod.SyncMod_commGlobal,
+        HOcommSchedule = k_mod.SyncMod_commSchedule\<rparr>\<close>)
+    hence "rho r q \<noteq> Aslept"
+        using stating[of "Suc r" rho q k HO sq] \<open>rho (Suc r) q = Active sq\<close>
+        by (metis SendVal.distinct(1) diff_Suc_1 k_mod.SyncMod_sendMsg_def run)
+    then obtain s where "rho r q = Active s" by (cases "rho r q") auto
+    moreover have "?msgs q = Content (Val (x sq))"
+        using HOrcvdMsgs_def[of ?A p "HO (Suc (Suc r)) p" "rho (Suc r)"] \<open>?msgs q = Content (Val v)\<close>
+        by (simp add: Active \<open>sendMsg (HOMachine_to_Algorithm (k_mod.SyncMod_HOMachine k)) q p sq = Val (x sq)\<close>)
+    ultimately have "rho r q = Active s \<and> rho (Suc r) q = Active sq \<and> x sq = v"
+        using \<open>rho (Suc r) q = Active sq\<close> \<open>?msgs q = Content (Val v)\<close> k_mod.SyncMod_sendMsg_def[of k q p sq] by auto
+    thus "\<exists>s ss. rho r q = Active s \<and> rho (Suc r) q = Active ss \<and> x ss = v"  by auto
+qed
 
+lemma transition : assumes s_def:"rho r p = Active s"
+and ss_def:"rho (Suc r) p = Active ss"
+and run:"HORun (HOMachine_to_Algorithm (k_mod.SyncMod_HOMachine k)) rho HO" (is "HORun ?A _ _")
+and "k > 2"
+shows "k_mod.SyncMod_nextState k p s (HOrcvdMsgs ?A p (HO (Suc r) p) (rho r)) ss" (is "k_mod.SyncMod_nextState  _ _ _ ?msgs _")
+and "x ss < k"
+proof -
+    have "CHOnextConfig ?A (rho r) (HO (Suc r)) (\<lambda>w. undefined) (rho (Suc r))" using run by (simp add:HORun_def CHORun_def)
+    then obtain sss where "rho (Suc r) p = Active sss \<and> CnextState ?A p s ?msgs undefined sss" 
+        using CHOnextConfig_def[of ?A "rho r" "HO (Suc r)" "\<lambda>w. undefined" "rho (Suc r)"] s_def by fastforce
+    hence "CnextState ?A p s ?msgs undefined ss" using ss_def by auto
+    hence nxt:"k_mod.SyncMod_nextState k p s ?msgs ss"
+        using HOMachine_to_Algorithm_def k_mod.SyncMod_HOMachine_def[of k] by (simp add:k_mod.simp_nextState)
+    hence "x ss < k"
+    proof (cases "k_mod.ready_force k ?msgs s")
+        case True
+        thus "x ss < k" using nxt k_mod.SyncMod_nextState_def \<open>k > 2\<close> by auto
+    next
+        case False
+        thus "x ss < k"
+        proof (cases "x ss = 0")
+            case True
+            thus "x ss < k" using \<open>k > 2\<close> by auto
+        next
+            case False
+            hence "(x ss) mod k = x ss" using nxt k_mod.SyncMod_nextState_def by auto
+            thus "x ss < k" using \<open>k > 2\<close> by (metis less_Suc_eq_0_disj less_imp_Suc_add mod_less_divisor)
+        qed
+    qed
+    thus "k_mod.SyncMod_nextState k p s ?msgs ss" and "x ss < k" using nxt by auto
+qed
 
 lemma A2 : assumes "k_mod.xi_nek HO xi"
 and run:"HORun (HOMachine_to_Algorithm (k_mod.SyncMod_HOMachine k)) rho HO" (is "HORun ?A _ _")
@@ -143,32 +168,154 @@ and run:"HORun (HOMachine_to_Algorithm (k_mod.SyncMod_HOMachine k)) rho HO" (is 
 and "rho r xi = Active s"
 and "x s = k - 1"
 and "k > 2"
-and "monovalent rho v r"
-shows "monovalent rho (v+i) (r+i)"
+and "monovalent rho (v mod k) r"
+shows "monovalent rho ((v+i) mod k) (r+i)"
 proof (induction i)
-    from assms(6) show \<open>monovalent rho (v+0) (r+0)\<close> by auto
+    from assms(6) show \<open>monovalent rho ((v+0) mod k) (r+0)\<close> by auto
 next
     case (Suc i)
+    let "?msgs p" = "(HOrcvdMsgs ?A p (HO (Suc (r+Suc i)) p) (rho (r+Suc i)))"
+    have no_discord:"\<forall>p q vv. ?msgs p q = Content (Val vv) \<longrightarrow> vv = (v+i) mod k"
+    proof (rule+)
+        fix p q vv
+        assume "?msgs p q = Content (Val vv)"
+        then obtain s ss where " rho (r+i) q = Active s \<and> rho (r+Suc i) q = Active ss \<and> x ss = vv"
+            using run sending[of k rho HO p "r+i" q vv] by auto
+        thus "vv = (v+i) mod k"
+            using Suc.IH monovalent_def[of rho "(v+i) mod k" "r+i"] by auto
+    qed
+
     have "rho (r+i) xi \<noteq> Aslept"
         using run HORun_def assms(3) nonAsleepAgain[of rho r xi ?A HO _ i] by (simp add: HORun_def add.commute)
     then obtain sx where "rho (r+i) xi = Active sx" by (cases "rho (r+i) xi") auto
     moreover have "rho (Suc (r+i)) xi \<noteq> Aslept"
         using run HORun_def assms(3) nonAsleepAgain[of rho r xi ?A HO _ "i+1"] by (simp add: HORun_def add.commute)
     then obtain sxx where "rho (Suc (r+i)) xi = Active sxx" by (cases "rho (Suc (r+i)) xi") auto
-    ultimately have "x sxx = v+i" using Suc.IH monovalent_def[of rho "v+i" "r+i" ] by auto
-    have "\<forall>p ss st. rho (r+Suc i) p = Active ss \<longrightarrow> rho (Suc (r+Suc i)) p = Active st \<longrightarrow> x st = v"
+    ultimately have "x sxx = (v+i) mod k" using Suc.IH monovalent_def[of rho "(v+i) mod k" "r+i" ] by auto
+    hence "\<forall>p. k_mod.SyncMod_sendMsg k xi p sxx = Val ((v+i) mod k)" using k_mod.SyncMod_sendMsg_def by 
+        (metis One_nat_def add_lessD1 assms(5) linorder_not_less mod_le_divisor mod_less_divisor
+        neq0_conv not_add_less2 numerals(2) plus_1_eq_Suc)
+    hence "\<forall>p. sendMsg ?A xi p sxx = Val ((v+i) mod k)"
+        using HOMachine_to_Algorithm_def k_mod.SyncMod_HOMachine_def by (simp add: k_mod.SyncMod_HOMachine_def)
+    hence "\<forall>p. ?msgs p xi = Content (Val ((v+i) mod k))" (is "\<forall>p. ?msgs p xi = _")
+        using assms(1) by (simp add: HOrcvdMsgs_def k_mod.xi_nek_def \<open>rho (Suc (r + i)) xi = Active sxx\<close>)
+
+    hence concord:"\<forall>p. k_mod.concordant (?msgs p) ((v+i) mod k)"
+        using k_mod.concordant_def[of _ "(v+i) mod k"] no_discord by smt
+
+    have "\<forall>p ss st. rho (r+Suc i) p = Active ss \<longrightarrow> rho (Suc (r+Suc i)) p = Active st \<longrightarrow> x st = (v + Suc i) mod k"
     proof (rule+)
         fix p ss st
         assume "rho (r+Suc i) p = Active ss" and "rho (Suc (r+Suc i)) p = Active st"
-        hence "k_mod.SyncMod_nextState k p ss (HOrcvdMsgs ?A p (HO (Suc (r+Suc i)) p) (rho (r+Suc i))) st"
-            (is "k_mod.SyncMod_nextState k p ss ?msgs st") using run by (simp add:transition)
-        show "x st = v"
-        proof (cases "k_mod.ready_force k ?msgs ss")
+        hence "k_mod.SyncMod_nextState k p ss (?msgs p) st" using run transition[of rho "r+Suc i" p ss st k HO] assms(5) by blast
+        show "x st = (v + Suc i) mod k"
+        proof (cases "k_mod.ready_force k (?msgs p) ss")
             case True
-            hence "\<exists>p1 p2 v1 v2. ?msgs p1 = Content (Val v1) \<and> ?msgs p2 = Content (Val v2) \<and> v1 \<noteq> v2"
+            hence "\<exists>p1 p2 v1 v2. (?msgs p) p1 = Content (Val v1) \<and> (?msgs p) p2 = Content (Val v2) \<and> v1 \<noteq> v2"
                 using k_mod.ready_force_def by blast
-            then obtain p1 p2 v1 v2 where "?msgs p1 = Content (Val v1)" and "?msgs p2 = Content (Val v2)" and "v1 \<noteq> v2" by auto
-            then obtain s1 s2 where "rho (r+Suc i) p1 = Active s1 \<and> x s1 = v1" and "rho (r+Suc i) p2 = Active s2 \<and> x s2 = v2"
-                using run sending[of k rho HO p "r+Suc i" p1 v1] sending[of k rho HO p "r+Suc i" p2 v2] by auto
-            hence ""
-    show "monovalent rho (v+Suc i) (r+Suc i)"
+            then obtain p1 p2 v1 v2 where "(?msgs p) p1 = Content (Val v1)" and
+                                          "(?msgs p) p2 = Content (Val v2)" and "v1 \<noteq> v2" by auto
+            then obtain s1 s2 ss1 ss2 where "rho (r+i) p1 = Active s1" and "rho (r+Suc i) p1 = Active ss1 \<and> x ss1 = v1" and
+                                            "rho (r+i) p2 = Active s2" and "rho (r+Suc i) p2 = Active ss2 \<and> x ss2 = v2"
+                using run sending[of k rho HO p "r+i" p1 v1] sending[of k rho HO p "r+i" p2 v2] by auto
+            hence "v1 = (v+i) mod k" and "v2 = (v+i) mod k" using Suc.IH monovalent_def[of rho "(v+i) mod k" "r+i"] by auto
+            thus "x st = (v + Suc i) mod k" using \<open>v1 \<noteq> v2\<close> by auto
+        next
+            case False
+            thus "x st = (v + Suc i) mod k"
+            proof (cases "x st = 0")
+                case True
+                hence "\<forall>vv. k_mod.concordant (?msgs p) vv \<longrightarrow> vv =  k - 1"
+                    using \<open>k_mod.SyncMod_nextState k p ss (?msgs p) st\<close> k_mod.SyncMod_nextState_def
+                    \<open>\<not> k_mod.ready_force k (?msgs p) ss\<close> by auto
+                hence "(v+i) mod k = k - 1" using concord k_mod.concordant_def by auto
+                thus "x st = (v+Suc i) mod k" using \<open>x st = 0\<close>
+                by (metis Suc_diff_1 assms(5) group_cancel.add2 less_imp_Suc_add mod_Suc_eq mod_self plus_1_eq_Suc zero_less_Suc)
+            next
+                case False
+                hence "k_mod.concordant (?msgs p) ((x st - 1) mod k)" and "(x st) mod k = x st"
+                    using \<open>k_mod.SyncMod_nextState k p ss (?msgs p) st\<close> k_mod.SyncMod_nextState_def
+                    \<open>\<not> k_mod.ready_force k (?msgs p) ss\<close> by auto
+                hence "(x st - 1) mod k = (v+i) mod k"
+                    using concord k_mod.concordant_def[of "?msgs p" ] by meson
+                thus "x st = (v+Suc i) mod k" using \<open>(x st) mod k = x st\<close>
+                    by (metis False add_diff_inverse_nat group_cancel.add2 mod_Suc_eq mod_by_1 mod_if plus_1_eq_Suc)
+            qed
+        qed
+    qed
+    thus "monovalent rho ((v+Suc i) mod k) (r+Suc i)" using monovalent_def[of rho "(v+Suc i) mod k" "r+Suc i"] by auto
+qed
+
+lemma A4 : assumes "k_mod.xi_nek HO xi"
+and run:"HORun (HOMachine_to_Algorithm (k_mod.SyncMod_HOMachine k)) rho HO" (is "HORun ?A _ _")
+and "rho r xi = Active s"
+and "x s = k - 1"
+and "k > 2"
+assumes commS:"HOcommSchedule (k_mod.SyncMod_HOMachine k) (Schedule rho)"
+shows "k_mod.liveness rho"
+proof -
+    have "\<exists>n. Schedule rho n = UNIV" using commS by (simp add:k_mod.SyncMod_HOMachine_def k_mod.SyncMod_commSchedule_def )
+    then obtain n :: nat where "!p. rho n p \<noteq> Aslept" by auto
+
+    have "monovalent rho 0 r" using A2 assms by auto
+    moreover have "(0+(n+1)*k-1) mod k = k-1"
+        by (smt Suc_diff_1 add.commute add.left_neutral add_diff_inverse_nat diff_Suc_1 diff_add_zero
+        mod_Suc mod_mult_self2_is_0 no_zero_divisors zero_eq_add_iff_both_eq_0 zero_neq_one)
+    ultimately have monoval:"monovalent rho ((k-1) :: nat) ((r+(n+1)*k-1) :: nat)" 
+        using A3[where ?v = 0 and ?i = "(n+1)*k-1" and ?r = r] assms 
+        by (metis (no_types, lifting) add.left_neutral less_one linorder_not_less mod_mult_self1 mod_mult_self2_is_0
+        no_zero_divisors not_less0 ordered_cancel_comm_monoid_diff_class.add_diff_assoc zero_eq_add_iff_both_eq_0)
+    have "\<forall>p r. rho r p \<noteq> Aslept --> (\<exists>rf sf. rho rf p = Active sf & fire sf)"
+    proof (rule allI impI)+
+        fix p
+        fix r :: nat
+        assume "rho r p \<noteq> Aslept"
+        moreover have "1 \<le> (n+1)*k" using \<open>k > 2\<close> by auto
+        hence "r+((n+1)*k-1) = r+(n+1)*k-1" (is "_ = ?rd") using  ordered_cancel_comm_monoid_diff_class.add_diff_assoc[of 1 "(n+1)*k" r] by auto
+        ultimately have "rho (Suc ?rd) p \<noteq> Aslept" using nonAsleepAgain[of rho r p _ _ _ "(n+1)*k"] run HORun_def
+            by (smt \<open>1 \<le> (n + 1) * k\<close> add.commute add_Suc_right ordered_cancel_comm_monoid_diff_class.add_diff_inverse plus_1_eq_Suc)
+        then obtain ss where "rho (Suc ?rd) p = Active ss" by (cases "rho (Suc ?rd) p") auto
+        moreover from this have "rho (Suc (Suc ?rd)) p \<noteq> Aslept"
+            using nonAsleepAgain[of rho "Suc ?rd" p _ _ _ 1] run HORun_def Suc_diff_1 assms(5) by fastforce
+        then obtain st where "rho (Suc (Suc ?rd)) p = Active st" by (cases "rho (Suc (Suc ?rd)) p") auto
+        ultimately have "k_mod.SyncMod_nextState k p ss (HOrcvdMsgs ?A p (HO (Suc (Suc ?rd)) p) (rho (Suc ?rd))) st"
+            (is "k_mod.SyncMod_nextState  _ _ _ ?msgs _")
+            using transition[of rho "Suc ?rd" p ss st] run assms(5) by auto
+        have "\<forall>q. ?msgs p = Void \<or> ?msgs p = Content (Val (k-1))"
+        proof
+            fix q
+            have "?rd-n = r+n*k+1*k-1-n" using \<open>k > 2\<close> by simp
+            hence positiv:"?rd-n > 0" using \<open>k > 2\<close>
+                by (metis add.commute add_lessD1 diff_diff_left mult.commute mult.right_neutral mult_less_cancel2
+                one_add_one trans_less_add2 zero_less_diff )
+            hence "rho ?rd q ~= Aslept"
+                using nonAsleepAgain[of rho n q ?A HO "\<lambda>r q. undefined" "?rd-n"]
+                run HORun_def[of ?A rho HO] \<open>\<forall>p. rho n p ~= Aslept\<close> \<open>k > 2\<close> by auto
+            then obtain sq where "rho ?rd q = Active sq" by (cases "rho ?rd q") auto
+            moreover have "rho (Suc ?rd) q ~= Aslept"
+                using run HORun_def[of ?A rho HO] \<open>k > 2\<close>
+                by (metis \<open>rho ?rd q ~= Aslept\<close> nonAsleepAgain plus_1_eq_Suc)
+            then obtain sqq where "rho (Suc ?rd) q = Active sqq" by (cases "rho (Suc ?rd) q") auto
+            moreover have "r+(n+1)*k > 0" using \<open>k > 2\<close> by auto
+
+
+            moreover have "monovalent rho ((k - 1) :: nat) (?rd :: nat)" using monoval by auto
+    
+
+
+                ultimately have "x sqq = k-1"
+                    using assms monovalent_def[of rho "k-1" ?rd] by auto
+
+                hence "k_mod.SyncMod_sendMsg k q p sqq = Val (k-1)"
+                    using k_mod.SyncMod_sendMsg_def[of k q p sqq] \<open>k > 2\<close> by auto 
+                hence "sendMsg ?A q p sqq = Val (k-1)"
+                    using k_mod.SyncMod_HOMachine_def HOMachine_to_Algorithm_def
+                    by (simp add: `\<And>k. k_mod.SyncMod_HOMachine k \<equiv> (| CinitState = \<lambda>p st crd. k_mod.SyncMod_initState k p st,
+                    sendMsg = k_mod.SyncMod_sendMsg k, CnextState = \<lambda>p st msgs crd. k_mod.SyncMod_nextState k p st msgs,
+                    HOcommPerRd = k_mod.SyncMod_commPerRd, HOcommGlobal = k_mod.SyncMod_commGlobal, HOcommSchedule = k_mod.SyncMod_commSchedule |)`)
+                hence "?msgs q = (if q : HO (Suc (Suc ?rd)) p then Content (Val (k-1)) else Void)"
+                    using HOrcvdMsgs_def[of ?A p "HO (Suc (Suc ?rd)) p" "rho (Suc ?rd)"] `rho (Suc ?rd) q = Active sqq` by auto
+                thus "?msgs q = Void \<or> ?msgs q = Content (Val (k-1))" by auto
+            qed
+
+        show "\<exists>rf sf. rho rf p = Active sf \<and> fire sf"
